prove generic call value checker packages

fixtures/TypeChecker.ml
@@ -8645,7 +8645,58 @@ let rec infer_core_env_state_fuel_roots fuel env _UU03a9_ n r _UU03a3_ e =
                 | _ -> Infer_err ErrNotImplemented)
              | Infer_err err -> Infer_err err)
           | Infer_err err -> Infer_err err))
-    | ECallExprGeneric (_, _, _) -> Infer_err ErrNotImplemented
+    | ECallExprGeneric (callee, type_args, args) ->
+      (match infer_core_env_state_fuel_roots fuel' env _UU03a9_ n r _UU03a3_
+               callee with
+       | Infer_ok p ->
+         let (p0, roots_callee) = p in
+         let (p1, r1) = p0 in
+         let (t_callee, _UU03a3_1) = p1 in
+         let collect =
+           let rec collect _UU03a3_0 r0 = function
+           | [] -> Infer_ok ((([], _UU03a3_0), r0), [])
+           | e' :: es ->
+             (match infer_core_env_state_fuel_roots fuel' env _UU03a9_ n r0
+                      _UU03a3_0 e' with
+              | Infer_ok p2 ->
+                let (p3, roots_e) = p2 in
+                let (p4, r2) = p3 in
+                let (t_e, _UU03a3_2) = p4 in
+                (match collect _UU03a3_2 r2 es with
+                 | Infer_ok p5 ->
+                   let (p6, roots_es) = p5 in
+                   let (p7, r3) = p6 in
+                   let (tys, _UU03a3_3) = p7 in
+                   Infer_ok ((((t_e :: tys), _UU03a3_3), r3),
+                   (roots_e :: roots_es))
+                 | Infer_err err -> Infer_err err)
+              | Infer_err err -> Infer_err err)
+           in collect
+         in
+         (match collect _UU03a3_1 r1 args with
+          | Infer_ok p2 ->
+            let (p3, arg_roots) = p2 in
+            let (p4, r') = p3 in
+            let (arg_tys, _UU03a3_') = p4 in
+            (match ty_core t_callee with
+             | TTypeForall (_, bounds, body) ->
+               (match ty_core body with
+                | TFn (param_tys, ret) ->
+                  (match check_type_forall_bounds env bounds type_args with
+                   | Some err -> Infer_err err
+                   | None ->
+                     (match check_arg_tys _UU03a9_ arg_tys
+                              (map (subst_type_params_ty type_args) param_tys) with
+                      | Some err -> Infer_err err
+                      | None ->
+                        Infer_ok ((((subst_type_params_ty type_args ret),
+                          _UU03a3_'), r'),
+                          (root_set_union roots_callee
+                            (root_sets_union arg_roots)))))
+                | x -> Infer_err (ErrMalformedHrtBody x))
+             | _ -> Infer_err ErrNotImplemented)
+          | Infer_err err -> Infer_err err)
+       | Infer_err err -> Infer_err err)
     | EStruct (sname, lts, args, fields) ->
       (match lookup_struct sname env with
        | Some s ->
@@ -11116,7 +11167,58 @@ let rec infer_core_env_state_fuel_roots_shadow_safe fuel env _UU03a9_ n r _UU03a
                 | _ -> Infer_err ErrNotImplemented)
              | Infer_err err -> Infer_err err)
           | Infer_err err -> Infer_err err))
-    | ECallExprGeneric (_, _, _) -> Infer_err ErrNotImplemented
+    | ECallExprGeneric (callee, type_args, args) ->
+      (match infer_core_env_state_fuel_roots_shadow_safe fuel' env _UU03a9_ n
+               r _UU03a3_ callee with
+       | Infer_ok p ->
+         let (p0, roots_callee) = p in
+         let (p1, r1) = p0 in
+         let (t_callee, _UU03a3_1) = p1 in
+         let collect =
+           let rec collect _UU03a3_0 r0 = function
+           | [] -> Infer_ok ((([], _UU03a3_0), r0), [])
+           | e' :: es ->
+             (match infer_core_env_state_fuel_roots_shadow_safe fuel' env
+                      _UU03a9_ n r0 _UU03a3_0 e' with
+              | Infer_ok p2 ->
+                let (p3, roots_e) = p2 in
+                let (p4, r2) = p3 in
+                let (t_e, _UU03a3_2) = p4 in
+                (match collect _UU03a3_2 r2 es with
+                 | Infer_ok p5 ->
+                   let (p6, roots_es) = p5 in
+                   let (p7, r3) = p6 in
+                   let (tys, _UU03a3_3) = p7 in
+                   Infer_ok ((((t_e :: tys), _UU03a3_3), r3),
+                   (roots_e :: roots_es))
+                 | Infer_err err -> Infer_err err)
+              | Infer_err err -> Infer_err err)
+           in collect
+         in
+         (match collect _UU03a3_1 r1 args with
+          | Infer_ok p2 ->
+            let (p3, arg_roots) = p2 in
+            let (p4, r') = p3 in
+            let (arg_tys, _UU03a3_') = p4 in
+            (match ty_core t_callee with
+             | TTypeForall (_, bounds, body) ->
+               (match ty_core body with
+                | TFn (param_tys, ret) ->
+                  (match check_type_forall_bounds env bounds type_args with
+                   | Some err -> Infer_err err
+                   | None ->
+                     (match check_arg_tys _UU03a9_ arg_tys
+                              (map (subst_type_params_ty type_args) param_tys) with
+                      | Some err -> Infer_err err
+                      | None ->
+                        Infer_ok ((((subst_type_params_ty type_args ret),
+                          _UU03a3_'), r'),
+                          (root_set_union roots_callee
+                            (root_sets_union arg_roots)))))
+                | x -> Infer_err (ErrMalformedHrtBody x))
+             | _ -> Infer_err ErrNotImplemented)
+          | Infer_err err -> Infer_err err)
+       | Infer_err err -> Infer_err err)
     | EStruct (sname, lts, args, fields) ->
       (match lookup_struct sname env with
        | Some s ->
