rocq/theories/TypeSystem/EnvStructuralRules.v
@@ -1371,6 +1371,15 @@ Inductive typed_env_structural (env : global_env) (Ω : outlives_ctx) (n : nat)
         (params_of_tys (map (subst_type_params_ty type_args) param_tys)) Σ' ->
       typed_env_structural env Ω n Σ (ECallExpr callee args)
         (subst_type_params_ty type_args ret) Σ'
+  | TES_CallExprGeneric_TypeForall :
+      forall Σ Σ1 Σ' callee args u m bounds body param_tys ret type_args,
+      typed_env_structural env Ω n Σ callee (MkTy u (TTypeForall m bounds body)) Σ1 ->
+      ty_core body = TFn param_tys ret ->
+      check_type_forall_bounds env bounds type_args = None ->
+      typed_args_env_structural env Ω n Σ1 args
+        (params_of_tys (map (subst_type_params_ty type_args) param_tys)) Σ' ->
+      typed_env_structural env Ω n Σ (ECallExprGeneric callee type_args args)
+        (subst_type_params_ty type_args ret) Σ'
   | TES_CallExpr_MakeClosure : forall Σ Σ' fname fdef captures env_lt
       captured_tys args σ,
       In fdef (env_fns env) ->
@@ -1533,6 +1542,18 @@ Inductive typed_env_roots (env : global_env) (Ω : outlives_ctx) (n : nat)
         (params_of_tys (map (subst_type_params_ty type_args) param_tys))
         Σ' R' arg_roots ->
       typed_env_roots env Ω n R Σ (ECallExpr callee args)
+        (subst_type_params_ty type_args ret_inner)
+        Σ' R' (root_set_union roots_callee (root_sets_union arg_roots))
+  | TER_CallExprGeneric_TypeForall : forall R R1 R' Σ Σ1 Σ' callee args u
+      type_params bounds body_ty param_tys ret_inner type_args arg_roots roots_callee,
+      typed_env_roots env Ω n R Σ callee
+        (MkTy u (TTypeForall type_params bounds body_ty)) Σ1 R1 roots_callee ->
+      ty_core body_ty = TFn param_tys ret_inner ->
+      check_type_forall_bounds env bounds type_args = None ->
+      typed_args_roots env Ω n R1 Σ1 args
+        (params_of_tys (map (subst_type_params_ty type_args) param_tys))
+        Σ' R' arg_roots ->
+      typed_env_roots env Ω n R Σ (ECallExprGeneric callee type_args args)
         (subst_type_params_ty type_args ret_inner)
         Σ' R' (root_set_union roots_callee (root_sets_union arg_roots))
   | TER_CallExpr_MixedForall : forall R R1 R' Σ Σ1 Σ' callee args u u_body
@@ -2387,6 +2408,30 @@ Proof.
     exists R0', (root_set_union roots_callee0 (root_sets_union arg_roots0)).
     split; [| split; [| split]].
     + eapply TER_CallExpr_TypeForall; eauto.
+    + exact HnsR0'.
+    + exact HR0'.
+    + eapply root_set_equiv_trans.
+      * apply root_set_union_equiv.
+       -- exact Hroots_callee0.
+       -- eapply root_set_equiv_trans.
+          ++ apply root_sets_union_equiv. exact Harg_roots0.
+          ++ apply root_set_equiv_sym. apply root_sets_instantiate_union_equiv.
+      * apply root_set_equiv_sym. apply root_set_instantiate_union_equiv.
+  - intros R R1 R' Σ Σ1 Σ' callee args u type_params bounds body_ty
+      param_tys ret_inner type_args arg_roots roots_callee
+      Hcallee IHcallee Hbody Htf_bounds Hargs IHargs Hfresh R0 HnsR HnsR0 HR0.
+    rewrite expr_local_store_names_call_expr_generic in Hfresh.
+    apply root_subst_images_exclude_names_app_inv in Hfresh.
+    destruct Hfresh as [Hfresh_callee Hfresh_args].
+    assert (HnsR1 : root_env_no_shadow R1).
+    { eapply typed_env_roots_no_shadow; [exact Hcallee | exact HnsR]. }
+    destruct (IHcallee Hfresh_callee R0 HnsR HnsR0 HR0)
+      as [R10 [roots_callee0 [Hcallee0 [HnsR10 [HR10 Hroots_callee0]]]]].
+    destruct (IHargs Hfresh_args R10 HnsR1 HnsR10 HR10)
+      as [R0' [arg_roots0 [Hargs0 [HnsR0' [HR0' Harg_roots0]]]]].
+    exists R0', (root_set_union roots_callee0 (root_sets_union arg_roots0)).
+    split; [| split; [| split]].
+    + eapply TER_CallExprGeneric_TypeForall; eauto.
     + exact HnsR0'.
     + exact HR0'.
     + eapply root_set_equiv_trans.
@@ -3355,6 +3400,8 @@ Proof.
         sctx_same_bindings_trans.
     + eauto using typed_args_env_structural_same_bindings,
         sctx_same_bindings_trans.
+	    + eauto using typed_args_env_structural_same_bindings,
+	      sctx_same_bindings_trans.
 	    + eauto using typed_args_env_structural_same_bindings,
 	      sctx_same_bindings_trans.
 	    + eauto using typed_args_env_structural_same_bindings,
